

**Solutions to Exercises from**  
***High-Dimensional Probability***

Roman Vershynin

Compiled by Hooman Zolfaghari

**Contents**

<b>1</b>	<b>Chapter 0</b>	<b>2</b>
<b>2</b>	<b>Chapter 1</b>	<b>2</b>
<b>3</b>	<b>Chapter 2</b>	<b>4</b>

## 1 Chapter 0

## 2 Chapter 1

*Exercise 2.1.*

**Solution.**

□

*Exercise 2.2.*

**Solution.**

$$f(x) := \max_i f_i(x) \quad f_i \text{ are convex functions}$$

$$\begin{aligned} f(\lambda x + (1 - \lambda)y) &= \max_i f_i(\lambda x + (1 - \lambda)y) \leq \\ &\max_i \lambda f_i(x) + (1 - \lambda)f_i(y) \leq \max_i \lambda f_i(x) + \max_i (1 - \lambda)f_i(y) = \lambda f(x) + (1 - \lambda)f(y) \end{aligned}$$

□

*Exercise 2.3.*

**Solution.**

1. induction on the definition
2. definition of expected value for discrete random variable

□

*Exercise 2.4.*

**Solution.** We know  $T \subseteq \text{conv}(T)$ , therefore  $\sup_{x \in T} f(x) \leq \sup_{x \in \text{conv}(T)} f(x)$ .

Also we have for some  $\epsilon > 0$  and  $S := \sup_{x \in \text{conv}(T)} f(x)$  that  $\exists y \in \text{conv}(T)$   $f(y) > S - \epsilon$ . Now  $y = \sum_{i=1}^m \lambda_i x_i$  for  $x_i \in T, \lambda \geq 0, \sum_{i=1}^m \lambda_i = 1$  which also means  $\lambda_i \leq 1$ . By convexity of  $f$  and Jensen's inequality we have:

$$f(y) \leq \sum_{i=1}^m \lambda_i f(x_i) \leq \max_{1 \leq i \leq m} f(x_i) \leq \sup_{x \in T} f(x)$$

So

$$[\forall \epsilon > 0 \quad S - \epsilon < f(y) \leq \sup_{x \in T} f(x)] \implies \sup_{x \in \text{conv}(T)} f(x) \leq \sup_{x \in T} f(x)$$

□

*Exercise 2.5.*

**Solution.** case  $n = 2$ :  $x = (x_1, x_2)$ ,  $x_i \in [0, 1]$ :

$$\begin{aligned} x &= (1 - x_2)(x_1(1, 0) + (1 - x_1)(0, 0)) + x_2(x_1(1, 1) + (1 - x_1)(0, 1)) \\ &= (1 - x_2)(x_1(1, 0) + (1 - x_2)(1 - x_2)(0, 0) + x_2(x_1(1, 1) + x_2(1 - x_1)(0, 1)) \end{aligned}$$

conjecture: For each  $v = (v_1, \dots, v_n) \in \{0, 1\}^n$  define:

$$\lambda_v := \prod_{i=1}^n [(v_i)(x_i) + (1 - v_i)(1 - x_i)]$$

proof by induction: We can verify for  $n = 1, 2$  as above. Assume this works for  $n = k - 1$ , meaning any point in  $[0, 1]^{k-1}$  can be written as  $x = \sum_{v \in \{0, 1\}^{k-1}} \lambda_v v$ . We can prove now for  $n = k$  by taking a choosing one of its dimensions and letting a hyper-surface orthogonal to that point create a  $k - 1$  dimensional cube. now we have  $\square$

*Exercise 2.6.*

*Exercise 2.7.*

*Exercise 2.8.*

**Solution.** We want to prove that with probability less than or equal to  $n$  there exists an independent group of size more than  $2 \log_2 n$ . We have  $n \geq 7$ , therefore  $\lfloor 2 \log_2 n \rfloor > 4$ . So we have the size  $k \geq 5$ .  $\square$

*Exercise 2.9.*

*Exercise 2.10.*

*Exercise 2.11.*

*Exercise 2.12.*

**Solution.**

1. An inequality that relates to different norms is Holder's inequality so we try to use that. We define  $r := \frac{q}{p}$ , where its conjugate is  $r' := 1/(1 - \frac{p}{q}) = \frac{q}{q-p}$ . We take the  $r$ -norm of  $X^p$  and  $r'$ -norm of 1 to see:

$$\begin{aligned} \|X^p\|_1 &\leq \|X^p\|_r \|1\|_{r'} = \|X^p\|_r \\ \implies \mathbb{E}|X^p| &\leq (\mathbb{E}|X|^q)^{p/q} \implies \text{answer} \end{aligned}$$

For  $0 \leq p < 1$  we should have used Jensen instead of Holder.

2. Recall  $\|X\|_{L^p} = (\mathbb{E}|X|^p)^{1/p}$ . For continuous  $X$  with distribution  $f$  we have  $\mathbb{E}|X|^p = \int_D |x|^p f(x) dx$ , where  $D$  is the domain of  $f$  (range of  $X$ ). Take  $\alpha = \frac{p+q}{2}$ . Now if we had  $f(x) = |x|^{-1-\alpha}$  then  $|x|^{p-1-\alpha}$  will converge (its exponent is  $\leq -1$ ) and  $|x|^{q-1-\alpha}$  will diverge. But we need to make sure  $f$  is a valid density function, i.e.  $\int_D f(x) dx = 1$ . To make things simpler we take  $X \geq 1$  so we can remove the absolute value functions. Now we have  $\int_1^\infty x^{-1-\alpha} dx = [x^{-\alpha}/-\alpha]_1^\infty = 1/\alpha$ . So we must define  $f_X(x) := \alpha x^{-1-\alpha}$ . Also for a discrete example we could create an infinite sum that converges diverges when its elements are gone to the powers more than  $p$  and converges otherwise.  $\square$

*Exercise 2.13.*

**Solution.**

□

### 3 Chapter 2

*Exercise 3.1.* (Products of i.i.d. random variables do not concentrate)

$$X_1, \dots, X_n \in \text{Uniform}([0, 1])$$

$$Y_n := X_1 \cdots X_n$$

**Solution.** Since  $X_i$  are independent:

$$\mathbb{E}[Y_n] = \prod_{i=1}^n \mathbb{E}[X_i] = \prod_{i=1}^n \int_0^1 x \, dx = 2^{-n}$$

$$\mathbb{P}[Y_n \geq \mathbb{E}Y_n] = \mathbb{P}[Y_n \geq 2^{-n}] \geq \mathbb{P}(Y_1 \geq \frac{1}{2} \wedge \cdots \wedge Y_n \geq \frac{1}{2}) = (0.5)^n$$

We also have:

$$\log Y_n = \sum_{i=1}^n \log X_i, \quad \log X_i \in (-\infty, 0]$$

$$\mathbb{P}[Y_n \geq \mathbb{E}Y_n] = \mathbb{P}\left(\sum_{i=1}^n \log X_i \geq -n \log 2\right) \leq$$

???

□

*Exercise 3.2.* (Gaussian tails: a lower bound)

**Solution.**

$$\mathbb{P}(g \geq t) = \int_t^\infty \frac{1}{\sqrt{2\pi}} e^{-x^2/2} \, dx, \quad \frac{d}{dt} \mathbb{P}(g \geq t) = -\frac{1}{\sqrt{2\pi}} e^{-t^2/2}$$

$$\frac{d}{dt} \frac{t}{t^2 + 1} \cdot \frac{1}{\sqrt{2\pi}} e^{-t^2/2} = \frac{1}{\sqrt{2\pi}} \left( \frac{1 - 2t^2 - t^4}{(t^2 + 1)^2} \right) e^{-t^2/2}$$

defining  $h(t) := \mathbb{P}(g \geq t) - \frac{t}{t^2 + 1} \cdot \frac{1}{\sqrt{2\pi}} e^{-t^2/2}$  we can see that

$$\frac{d}{dt} h(t) = \frac{-2}{(t^2 + 1)^2 \sqrt{2\pi}} e^{-t^2/2}$$

. We have  $h'(t) < 0$  for all  $t$ . and  $\lim_{t \rightarrow \infty} h'(t) = 0$ . So the function  $h(t)$  is strictly decreasing. We can also verify that  $h(0) > 0$  and  $\lim_{t \rightarrow \infty} h(t) = 0$ , so the function cannot become negative at any point  $t$ .

□

*Exercise 3.3.* (Mills ratio)

*Exercise 3.4.* (Truncated Gaussian moments)

**Solution.**

1.

$$\mathbb{E}[g\mathbf{1}_{g>t}] = \frac{1}{\sqrt{2\pi}} \int_{-\infty}^{\infty} x\mathbf{1}_{x>t} e^{-x^2/2} dx = \frac{1}{\sqrt{2\pi}} \int_t^{\infty} x e^{-x^2/2} dx = \frac{1}{\sqrt{2\pi}} [-e^{-x^2/2}]_t^{\infty} = \frac{1}{\sqrt{2\pi}} e^{-t^2/2}$$

2.

$$\mathbb{E}[g^2\mathbf{1}_{g>t}] = \frac{1}{\sqrt{2\pi}} \int_t^{\infty} x^2 e^{-x^2/2} dx$$

Integration by parts  $u := x$  and  $v := e^{-x^2/2}$  gives:

$$\leq \frac{1}{\sqrt{2\pi}} (te^{-t^2/2} + \int_t^{\infty} e^{-x^2/2} dx) \leq \frac{1}{\sqrt{2\pi}} (te^{-t^2/2} + \frac{1}{t}e^{-t^2/2}) = \frac{1}{\sqrt{2\pi}} (t + \frac{1}{t})e^{-t^2/2}$$

□

*Exercise 3.5.* (Completing the proof of Hoeffding inequality)

**Solution.** Taylor expansion

□

*Exercise 3.6.* (Gaussian tail by the exponential moment method)

**Solution.** for any  $t \geq 0$ :

$$\begin{aligned} \mathbb{P}(g \geq t) &= \mathbb{P}(e^{\lambda g} \geq e^{\lambda t}) \leq e^{-\lambda t} \mathbb{E}[e^{\lambda g}] \\ &= e^{-\lambda t} \int_{-\infty}^{\infty} e^{\lambda x} \frac{1}{\sqrt{2\pi}} e^{-x^2/2} dx = e^{-\lambda t} \int_{-\infty}^{\infty} \frac{1}{\sqrt{2\pi}} e^{\frac{\lambda^2 - (x-\lambda)^2}{2}} dx \\ &= e^{-\lambda t + \lambda^2/2} \int_{-\infty}^{\infty} \frac{1}{\sqrt{2\pi}} e^{\frac{-(x-\lambda)^2}{2}} dx = e^{-\lambda t + \lambda^2/2} \end{aligned}$$

$$\text{minimize by setting } \lambda = t \implies \mathbb{P}(g \geq t) \leq e^{-t^2/2}$$

□

*Exercise 3.7.* (Small ball probability)

**Solution.**

$$\mathbb{P}(\sum_{i=1}^N X_i \leq \epsilon N) = \mathbb{P}(e^{\lambda \sum_{i=1}^N X_i} \leq e^{\lambda \epsilon N}) \leq e^{-\lambda \epsilon N} \prod_{i=1}^N \mathbb{E}[e^{\lambda X_i}] = e^{-\lambda \epsilon N} \prod_{i=1}^N$$

□